Change Name to be string in schema and add docs to schema related things
Not sure what to do with the lemmas about schema wf... which may not make much
sense.

src/SchemaWellFormedness.v
@@ -2,6 +2,7 @@ From mathcomp Require Import all_ssreflect.
 Set Implicit Arguments.
 Unset Strict Implicit.
 Unset Printing Implicit Defensive.
+From CoqUtils Require Import string.
 From extructures Require Import ord fset fmap.
 
 From Equations Require Import Equations.
@@ -15,57 +16,52 @@ Require Import SchemaAux.
 
 Section WellFormedness.
 
-  Variables (Name Vals : ordType).
+  Variables (Vals : eqType).
 
   Section Defs.
     
-    Variable (s : @schema Name).
+    Variable (s : graphQLSchema).
 
     
-    (** Subtype relation
+    (** ** Subtyping relation.
+        Using Schema as the lookup function in the schema (Schema : Name -> TypeDefinition).
 
    
-                 ----------------------- (ST_Refl)
+                 [-----------------------] (ST_Refl) #<br>#
                        ty <: ty
 
                   
-       Doc(O) = type O implements ... I ... { ... }
-                Doc(I) = interface I { ...}
+       Schema(O) = type O implements ... I ... { ... }
+                Schema(I) = interface I { ...}
        ------------------------------------------- (ST_Object)
                          O <: I
 
            
                          T <: U
-                ------------------------- (ST_ListType)
+                [-------------------------] (ST_ListType)
                        [T] <: [U]
+                       
 
+    ----
+    **** Observations
 
-    Some observations:
-        1. Transitivity : There is no need to specify this because only objects can 
-        be subtype of an interface and not between objects. Interfaces cannot be
-        subtype of another interface.
-     **)
-    Inductive Subtype : type -> type -> Prop :=
-    | ST_Refl : forall ty, Subtype ty ty
-                              
-    | ST_Interface : forall n n',
-        declares_implementation s n n' ->
-        Subtype (NT n) (NT n')
-                
-    | ST_Union : forall n n',
-        (n \in (union_members s n')) ->
-        Subtype (NT n) (NT n')
-                
-    | ST_ListType : forall ty ty',
-        Subtype ty ty' ->
-        Subtype [ ty ] [ ty' ]. 
+        1. Limitations : Subtyping is strictly between objects and interfaces.
+           There cannot be an object that is subtype of another, as well as an
+           interface implementing another interface.
 
+        2. Transitivity : Because of the limitation, there is no need to specify
+           or worry about transitivity of the relation.
+
+        #<a href='https://graphql.github.io/graphql-spec/June2018/##sec-Objects'> See also: Object Type Validation subsection </a>#
+
+        #<a href='https://graphql.github.io/graphql-spec/June2018/##sec-Interfaces'> See also: Interface Type Validation subsection </a>#
+    *)
     Reserved Infix "<:" (at level 60).
-    Equations is_subtype (ty ty' : @type Name) : bool :=
+    Equations is_subtype (ty ty' : type) : bool :=
       {
         [ lty ] <: [ lty' ] := lty <: lty';
 
-        NT name <: NT name' :=
+        NamedType name <: NamedType name' :=
           [|| (name == name'),
            declares_implementation s name name' | 
            (name \in (union_members s name'))];
@@ -77,201 +73,289 @@ Section WellFormedness.
     
     
     
-    (** The two following definitions describe whether a given type is a valid type
-      for a field argument (IsValidArgumentType) and if it is a valid type for a field itself 
-      (IsValidFieldType).
+    (** ** Valid argument's type
 
-      In the spec they are correspondently named "IsInputField" and "IsOutputField".
+        The following definition describe whether a given type is valid
+        for a field argument.
 
-      https://facebook.github.io/graphql/June2018/#sec-Input-and-Output-Types **)
+        In the spec it is named "IsInputType" but here it is renamed to make it more clear
+        that it is a check on the argument's type.
 
-    Inductive valid_argument_type  : type -> Prop :=
-    | VScalar_Arg : forall ty,
-        is_scalar_type s ty ->
-        valid_argument_type (NT ty)
-    | VEnum_Arg : forall ty,
-        is_enum_type s ty ->
-        valid_argument_type (NT ty)
-    | VList_Arg : forall ty,
-        valid_argument_type ty ->
-        valid_argument_type (ListType ty).
+        Observations:
+
+        1. InputObject : The spec allows the Input Object type as well as the
+           scalar and enum types, but since we are not currently implementing it, 
+           we discard it in this definition.
+
+        2. Non-Null type : Similarly as the previous point.
+
+        https://graphql.github.io/graphql-spec/June2018/#sec-Input-and-Output-Types
+        https://graphql.github.io/graphql-spec/June2018/#sec-Field-Arguments
+        https://graphql.github.io/graphql-spec/June2018/#sec-Objects (Section 'Type Validation')
+        https://graphql.github.io/graphql-spec/June2018/#sec-Interfaces (Section 'Type Validation')
+    *)
+    Equations is_valid_argument_type (ty : type) : bool :=
+      {
+        is_valid_argument_type [ ty ] := is_valid_argument_type ty;
+        is_valid_argument_type (NamedType name) := is_scalar_type s name || is_enum_type s name
+      }.
+
+
+    (** ** Valid field's return type 
+        
+        The following definition describe whether a given type is valid
+        for a field's return type.
+
+        In the spec it is named "IsOutputType" but here it is renamed to make it more clear
+        that it is a check on the field's return type.
+
+        Observations:
+
+        1. InputObject : The spec does not allow Input Object type to be
+           a valid return type but since we are not implementing it, we
+           simply ignore it. This allows for every other type to be a valid
+           return type (as long as it is declared in the schema).
+
+        https://graphql.github.io/graphql-spec/June2018/#sec-Input-and-Output-Types
+        https://graphql.github.io/graphql-spec/June2018/#sec-Objects (Section 'Type Validation')
+        https://graphql.github.io/graphql-spec/June2018/#sec-Interfaces (Section 'Type Validation')
+    *)
+    Equations is_valid_field_type (ty : type) : bool :=
+      {
+        is_valid_field_type [ ty ] := is_valid_field_type ty;
+        is_valid_field_type (NamedType name) := is_declared s name
+      }.
     
-    Fixpoint is_valid_argument_type  (ty : type) : bool :=
-      match ty with
-      | NT name => is_scalar_type s ty || is_enum_type s ty
-      | [ ty' ] => is_valid_argument_type  ty'
-      end.
 
+    (** ** Argument Well-formedness
 
-    
-    (* Because we are not considering InputObjects, a field may have any type, 
-     as long as it is declared in the Schema. *)
-    Inductive valid_field_type  : type -> Prop :=
-    | VBase_Type : forall n,
-        is_declared s n ->
-        valid_field_type (NT n)      
-    | VList_Type : forall ty,
-        valid_field_type ty ->
-        valid_field_type (ListType ty).
-    
-    Fixpoint is_valid_field_type (ty : type) : bool :=
-      match ty with
-      | NT n => is_declared s n
-      | [ ty' ] => is_valid_field_type  ty'
-      end.
-    
+      It checks whether an argument definition is well-formed by checking that
+      its type is a valid type for an argument. 
 
-    (** 
-      It checks whether an argument is well-formed by checking that
-      its type is a valid type for an argument **)
-    Definition is_field_argument_wf (arg : FieldArgumentDefinition) : bool :=
+      Observations:
+      1. Introspection : There is no check as to whether the argument's name 
+         begins with '__' because introspection is not implemented in this 
+         formalisation.
+
+      https://graphql.github.io/graphql-spec/June2018/#sec-Field-Arguments
+      https://graphql.github.io/graphql-spec/June2018/#sec-Objects (Section 'Type Validation')
+      https://graphql.github.io/graphql-spec/June2018/#sec-Interfaces (Section 'Type Validation')
+    *)
+    Definition is_wf_field_argument (arg : FieldArgumentDefinition) : bool :=
       is_valid_argument_type arg.(argtype).
 
     
-    (**
-     It states whether a field is well-formed.
+    (** ** Field Well-formedness
 
-                 ty isValidFieldType
-                  NoDuplicates args
-           ∀ arg ∈ args, arg isWellFormed
-           ------------------------------
-           (fname (args) : ty) isAWellFormedField
-     **)
-    Definition is_field_wf (fld : FieldDefinition) : bool :=
-      is_valid_field_type fld.(return_type) &&
-                                            (* uniq [seq arg.(argname) | arg <- fld.(fargs)] &  // Not specified... But should be? *)
-                                            all (is_field_argument_wf) fld.(fargs).
+     It checks whether a field is well-formed, independently of the type where it is
+     defined:
+
+     - It's return type is valid.
+     - There are no two arguments with the same name.
+     - All of its arguments are well-formed.
 
 
+     Observations:
+     1. Introspection : There is no check as to whether the argument's name 
+         begins with '__' because introspection is not implemented in this 
+         formalisation.
+     2. Argument's uniqueness : We could not find a reference in the spec
+        stating whether it is valid or not to have repeated arguments
+        but we are including this notion in this definition.
+               
+    *)
+    Definition is_wf_field (fld : FieldDefinition) : bool :=
+      [&& is_valid_field_type fld.(return_type),
+          uniq [seq arg.(argname) | arg <- fld.(fargs)] &  (* Not currently in the spec *)
+          all is_wf_field_argument fld.(fargs)].
 
-    (** This checks whether an object field is valid w/r to another from an implemented interface.
-      It checks the following:
+
+
+    (** ** Valid field implementation
+
+    This checks whether a field is valid w/r to another. This is used to check 
+    whether an Object type is correctly implementing an interface's fields.
+    
+    It checks the following:
       1. Both fields have the same name.
-      2. The arguments of the interface field must be a subset of the object's arguments.
+      2. The arguments of the interface field must be a subset of the object's arguments
+         (the types of the arguments are invariant, therefore we can simply check that it's a subset).
       3. The object's field return type must be a subtype of the interface's field.
 
-      This is not checking that any additional argument in the object must be a "non-required" field.
-     **)
-    Definition is_field_ok (fld fld' : FieldDefinition) : bool :=
-      [&& (fld.(fname) == fld'.(fname)),
-       fsubset fld'.(fargs) fld.(fargs) &
-       fld.(return_type) <: fld'.(return_type)].
+     
+    Observations:
+    1. Non-null extra arguments : The spec requires that any additional argument included in the object's
+       field must not be of a non-null type. Since we do not implement non-null types, we are not including 
+       this check. 
+    2. J&O : In Jorge and Olaf's paper, there is no check regarding arguments between an object 
+       type and its interface.
+
+      https://graphql.github.io/graphql-spec/June2018/#sec-Objects (Section 'Type Validation')
+    *)
+    Definition is_valid_field_implementation (object_field interface_field : FieldDefinition) : bool :=
+      [&& object_field.(fname) == interface_field.(fname),
+          subseq interface_field.(fargs) object_field.(fargs) &   (* I think this is wrong... *)
+          object_field.(return_type) <: interface_field.(return_type)].
     
 
 
 
     
-    (**
-     This checks whether an object type implements correctly an interface, 
-     by properly defining every field defined in the interface.
+    (** ** Valid interface implementation
+
+     This checks whether an object type correctly implements an interface, 
+     by properly implementing every field defined in the interface.
+     Using Schema as the lookup function in the schema (Schema : Name -> TypeDefinition).
 
 
             Schema(O) = type O implements ... I ... { Flds }   
                     Schema(I) = interface I { Flds' }
-                 ∀ fld' ∈ Flds', ∃ fld ∈ Flds s.t fld OK fld'
+      ∀ ifld ∈ Flds', ∃ ofld ∈ Flds s.t ofld is_valid_field_implementation ifld
             ------------------------------------------------
-                        O implementsOK I
+                        O implements_correctly I
 
-     **)
-    
-    Definition implements_interface_correctly (ty ty' : NamedType) : bool :=
-      let ifields := fields s ty' in
-      let ofields := fields s ty in
-      all (fun f' => has (fun f => is_field_ok f f') ofields) ifields.
+
+     Observations:
+     1. Implementation : From an implementation point of view, this definition might seem
+        a bit redundant (considering its posterior use). For the moment it is left here 
+        for readibility purposes.
+     *)
+    Definition implements_interface_correctly (object_type interface_type : Name) : bool :=
+      let interface_fields := fields s interface_type in
+      let object_fields := fields s object_type in
+      all (fun ifld => has (fun ofld => is_valid_field_implementation ofld ifld) object_fields) interface_fields.
     
 
     
-    (**
+    (** ** TypeDefinition Well-formedness
+        Using Schema as the lookup function in the schema (Schema : Name -> TypeDefinition).
+
 
                        Schema(S) = scalar S 
                        -----------------------
-                           scalar S OK
+                           scalar S is_wf_type_def
 
 
-                 Schema(O) = type O implements Ifs { Flds }
-                           notEmpty Flds
-                         NoDuplicates Flds
-                            Flds OK in O
-                            Ifs OK in O
+                 Schema(O) = Object O implements Intfs { Flds }
+                           Flds ≠ ∅
+                           Flds are_unique
+                    ∀ field ∈ Flds, field is_wf_field
+                           Intfs are_unique
+                  ∀ intf ∈ Intfs, S(intf) = interface intf { ... }
+                  ∀ intf ∈ Intfs, O implements_interface_correctly intf 
                 -----------------------------------------
-                          type O { Flds } 
+                  Object O implements Intfs { Flds } is_wf_type_def
 
 
 
                     Schema(I) = interface I { Flds }
-                           notEmpty Flds
-                         NoDuplicates Flds
-                            Flds OK in I
+                           Flds ≠ ∅
+                          Flds are_unique
+                         ∀ field ∈ Flds, field is_wf_field
                 ----------------------------------------
-                        interface I { Flds } 
+                        interface I { Flds }  is_wf_type_def
 
 
 
                        Schema(U) = union U { Mbs }
-                           notEmpty Mbs
-                         NoDuplicates Mbs
-                     ∀ mb ∈ Mbs, mb ObjectType
+                           Mbs ≠ ∅
+                         Mbs are_unique
+                     ∀ mb ∈ Mbs, Schema(mb) = Object mb implements ... { ... }
                 -----------------------------------------
-                          union U { Mbs } 
+                          union U { Mbs } is_wf_type_def
 
 
                        Schema(E) = enum E { Evs }
-                           notEmpty Evs
-                         NoDuplicates Evs
+                           Evs ≠ ∅
+                          Evs are_unique
                 -----------------------------------------
                           enum E { Evs } 
 
-     **)
-    
 
-    Fixpoint is_type_def_wf (tdef : TypeDefinition) : bool :=
+
+     Observations:
+     1. Enums : The spec does not specify whether the enum members must be different from 
+        other defined types in the schema (eg. Object type 'Human' cannot be part of a 
+        defined Enum type).
+     
+
+     https://graphql.github.io/graphql-spec/June2018/#sec-Scalars
+     https://graphql.github.io/graphql-spec/June2018/#sec-Objects (Section 'Type Validation')
+     https://graphql.github.io/graphql-spec/June2018/#sec-Interfaces (Section 'Type Validation')
+     https://graphql.github.io/graphql-spec/June2018/#sec-Unions (Section 'Type Validation')
+     https://graphql.github.io/graphql-spec/June2018/#sec-Enums (Section 'Type Validation')
+     *)
+    Fixpoint is_wf_type_def (tdef : TypeDefinition) : bool :=
       match tdef with
       | Scalar _ => true
                                    
       | Object name implements interfaces { fields } =>
-        [&& (fields != [::]),
-         uniq [seq fld.(fname) | fld <- fields],
-         all (is_field_wf) fields,
-         all (is_interface_type s) interfaces &
-         all (implements_interface_correctly name) interfaces]
-
+        [&& fields != [::],
+            uniq [seq fld.(fname) | fld <- fields],
+            all is_wf_field fields,
+            uniq interfaces,
+            all (is_interface_type s) interfaces &
+            all (implements_interface_correctly name) interfaces]
+ 
       | Interface _ { fields } =>
-        [&& (fields != [::]),
-         uniq [seq fld.(fname) | fld <- fields] &
-         all (is_field_wf) fields]
+        [&& fields != [::],
+            uniq [seq fld.(fname) | fld <- fields] &
+            all is_wf_field fields]
 
       | Union name { members } =>
-        (members != fset0) && all (is_object_type s) members
+        [&& members != [::],
+            uniq members &
+            all (is_object_type s) members]
 
-      | Enum _ { enumValues } => enumValues != fset0
+      | Enum _ { enumValues } => enumValues != [::]
                                                      
       end.
 
 
     
-    
-    Definition is_schema_wf : bool :=
-      [&& s.(query_type) \in s.(schema_names),
-                             is_object_type s s.(query_type),
-                             all (fun p => has_name p.1 p.2) s.(type_definitions) &
-                             all (fun p => is_type_def_wf p.2) s.(type_definitions)].
+    (** *** Schema Well-formedness 
+
+    This checks whether a schema is well-formed. 
+    1. The Query root operation is actually defined in the schema.
+    2. The Query type is an Object type.
+    3. Every type definition is well-formed 
+
+    Observations:
+
+    1. J&O : In Jorge and Olaf's paper, they describe a schema as being 'consistent'
+       if "every object type that implements an interface type i defines at least all 
+       the fields that i defines". Because they work with functions and sets they can 
+       simplify some checks about uniqueness of names, etc. Their notion does not capture, 
+       I believe, that fields' arguments between an object type and its interface have 
+       to satisfy some property (being a subset of the other).
+       
+    *)
+    Definition is_wf_schema : bool :=
+      [&& s.(query_type) \in s.(schema_names),      (* This is a bit redundant with the check about Query ∈ Ot *)
+          is_object_type s s.(query_type) &
+          all is_wf_type_def s.(type_definitions)].
 
   End Defs.
   
-  
-  Structure wfSchema := WFSchema {
-                           sch : @schema Name;
-                           hasType :  Name -> Vals -> bool;
-                           _ : is_schema_wf sch;
+
+  (** *** Well-formed Schema
+
+  A well-formed schema is a schema which satisfies the well-formedness property.
+  We also include the predicate "has_type", which 
+   *)
+  Structure wfGraphQLSchema := WFGraphQLSchema {
+                           schema : graphQLSchema;
+                           has_type :  Name -> Vals -> bool;
+                           _ : is_wf_schema schema;
                          }.
 
   
-  Coercion sch : wfSchema >-> Schema.schema.
+  Coercion schema : wfGraphQLSchema >-> graphQLSchema.
 
 
 End WellFormedness.
 
 
-Arguments wfSchema [Name Vals].
+Arguments wfGraphQLSchema [Vals].
 
 Infix "<:" := is_subtype (at level 50) : schema_scope.
